\documentclass[preview,12pt]{article}
\usepackage{amsmath}
\usepackage{gensymb}
\usepackage{ragged2e}
\usepackage{geometry}
\usepackage{graphicx}
\usepackage{caption}
\usepackage{subcaption}
\usepackage{pdfpages}

\geometry{letterpaper, margin=1in}

\begin{document}

\noindent PDE and Fourier\newline
Josh Coffey \newline
Homework 5 \newline
4/22/2020 \newline

\section*{(1)}
    Use the Fourier Transform to solve the following problem:
    $$u_t+u_x=0 \textrm{ with } u(x,0)=\frac{2}{x^2+1}$$
    \subsection*{(a)}
        Find the Fourier Transform of $u$ by applying $F$ to the equation and initial condition; denote this function $U(\omega,t).$
        $$F=\frac{1}{2\pi}\int_{-\infty}^\infty e^{iwx}f(x)dx$$
        $$F\{u_t\}+F\{u_x\}=0$$
        $$\frac{\partial}{\partial t}U(w,t)+iwU(w,t)=0$$
        This is now a linear, homogeneous ODE. Solving using integrating factor gives that:
        $$U(w,t)=A(w)e^{-iwt}$$
        Can calculate $A$ by taking the Fourier Transform of the IC.
        $$F\{u(x,0)\}=F\{\frac{2}{x^2+1}\}$$
        $$F\{\frac{2}{x^2+1}\}=\frac{1}{2\pi}\int_{-\infty}^\infty e^{iwx}\frac{2}{x^2+1}dx$$
        Using the table of inverse and forward Fourier Transforms given in the lectures where $\alpha=1$, 
        $$F\{\frac{2}{x^2+1}\}=e^{-|w|}$$
        Using this and plugging $t=0$ into $U(w,t)$ gives that $A(w)=e^{-|w|}$, and the full solution is that
        $$U(w,t)=e^{-|w|}e^{-iwt}$$
    \subsection*{(b)}
        Taking the inverse Fourier Transform of both sides to arrive at the solution of the original PDE gives:
        $$f(U(w,t))=f(e^{-|w|}e^{-iwt})=f(e^{-|w|-iwt})=f(e^{-|w|(1+it)})$$
        Using the table where $\alpha=(1+it)$ gives 
        $$u(x,t)=\frac{2(1+it)}{x^2+(1+it)^2}$$
        
\section*{(2)}
    Use the Fourier Transform to solve the following integro-differential equation:
    $$\sqrt{\pi}\int_R u_{tt}(s,t)e^{\frac{-(x-s)^2}{4}}ds=\sqrt{\frac{\pi}{3}}e^{\frac{-x^2}{12}}$$
    with initial conditions
    $$u(x,0)=0 \textrm{ and } u_t(x,0)=P_a(x)$$
    Where $P_a(x)=$
    \[ \begin{cases} 
      1 & |x|<a \\
      0 & otherwise \\
        \end{cases}
    \]
    Know that the left side of the integro-differential equation is the convolution of $u_{tt}$ and $e^\frac{-z^2}{4}$ \newline
    Taking the Fourier Transform of both sides gives:
    $$F\{(f*g)(w)\}=F\{\sqrt{\pi}\int_R u_{tt}(s,t)e^{\frac{-(x-s)^2}{4}}ds\}=F\{\sqrt{\frac{\pi}{3}}e^{\frac{-x^2}{12}}\}$$
    Know that taking the Fourier Transform of a convolution gives that:
    $$2\pi F\{f(w)\}F\{g(w)\}=2\pi F\{u_{tt}\} F\{\sqrt{\pi}e^{\frac{-(x-s)^2}{4}}\}=F\{\sqrt{\frac{\pi}{3}}e^{\frac{-x^2}{12}}\}$$
    Know from table that
    $$F\{u_{tt}\}=\frac{\partial^2 }{\partial t^2}U(w,t)$$
    $$F\{\sqrt{\pi}e^{\frac{-(x-s)^2}{4}}\}=e^{-w^2}$$
    $$F\{\sqrt{\frac{\pi}{3}}e^{\frac{-x^2}{12}}\}=e^{-3w^2}$$
    This gives the following equation:
    $$2\pi\frac{d^2U}{dt^2}e^{-w^2}=e^{-3w^2}$$
    $$\frac{d^2U}{dt^2}(w,t)=e^{-3w^2+w^2}=\frac{1}{2\pi}e^{-2w^2}$$
    Solving this ODE gives:
    $$y_h=0$$
    Guessing that $y_p=P_a(x)t$ gives that 
    $$U(w,t)=P_a(w)t$$
    Now take the inverse Fourier Transform to get
    $$u(x,t)=P_a(x)t$$
    
\section*{(3)}
    Consider the one-dimensional Schrodinger Problem:
    $$u_t=iu_{xx} \textrm{ with } u(x,0)=f(x)$$
    Where both $f$ and $u$ tend to 0 as $x->\pm \infty$
    \subsection*{(a)}
        Find the Fourier Transform in x of $u$ by applying $F$ to the equation and initial condition.  Denote this function $U=U(w,t).$
        $$F\{u_t\}=F\{iu_{xx}\}$$
        $$\frac{\partial U}{\partial t}=i(-iw)^2U=iw^2U$$
        Taking the Fourier Transform of the initial condition gives
        $$F\{u(x,0)\}=F\{f(x)\}$$
        $$U(w,0)=F\{f(w)\}$$
        Solving the new ODE for $U(w,t)$ 
        $$\frac{U'}{U}=iw^2$$
        $$\frac{dU}{U}=iw^2dt$$
        $$ln(U)=iw^2t+C$$
        $$U=Ae^{iw^2t}$$
        Using IC's:
        $$U(w,t)=F\{f(w)\}e^{iw^2t}$$
    \subsection*{(b)}
        Plancheral's Identity states
        $$\int_{-\infty}^\infty |g(x)|^2dx=2\pi\int_{-\infty}^\infty|G(w)|^2dw$$
        Show that 
        $$\int_{-\infty}^\infty |u(x,t)|^2dx=\int_{-\infty}^\infty|f(x)|^2dx$$
        Begin by taking the inverse Fourier Transform of $U(w,t)$
        $$F^{-1}\{U(w,t)\}=F^{-1}\{F\{f(w)\}e^{iw^2t}\}$$
        $$u(x,t)=f(x)F^{-1}\{e^{iw^2t}\}$$
        $$\int_{-\infty}^\infty|u(x,t)|^2dx=\int_{-\infty}^\infty|f(x)F^{-1}\{e^{iw^2t}\}|^2dx$$
        Using Plancheral's Identity:
        $$\int_{-\infty}^\infty |F^{-1}\{e^{iw^2t}\}|^2 dx=2\pi\int_{-\infty}^\infty |e^{iw^2t}|^2dw$$
        This integration results in the erf function which is equal to 1 at $\pm\infty$
        Thus 
        $$\int_{-\infty}^\infty |u(x,t)|^2dx=\int_{-\infty}^\infty|f(x)|^2dx$$
\end{document}
